ironfleet/src/Dafny/Distributed/Common/Framework/AbstractService.s.dfy
@@ -7,6 +7,7 @@ include "Environment.s.dfy"
 abstract module AbstractService_s {
 import opened Native__Io_s
 import opened Environment_s 
+import opened Native__NativeTypes_s
 
 type ServiceState 
 
