ironfleet/src/Dafny/Distributed/Common/Native/Io.s.dfy
@@ -136,7 +136,7 @@ class UdpClient
     ghost var env:HostEnvironment;
     function{:axiom} LocalEndPoint():EndPoint reads this;
     function{:axiom} IsOpen():bool reads this;
-    constructor{:axiom} () requires false;
+    constructor{:axiom} () {}//requires false;
 
     static method{:axiom} Construct(localEP:IPEndPoint, ghost env:HostEnvironment)
         returns(ok:bool, udp:UdpClient)
@@ -209,7 +209,7 @@ class FileSystemState
 {
 }
 
-class MutableSet<T(==)>
+class MutableSet<T(0,==,!new)>
 {
     static function method {:axiom} SetOf(s:MutableSet<T>) : set<T>
         reads s;
