ironfleet/src/Dafny/Distributed/Protocol/Common/NodeIdentity.i.dfy
@@ -1,7 +1,7 @@
 include "NodeIdentity.s.dfy"
 include "../../Common/Native/Io.s.dfy"
 
-module Concrete_NodeIdentity_i exclusively refines Common__NodeIdentity_s {
+module Concrete_NodeIdentity_i refines Common__NodeIdentity_s {
     import opened Native__Io_s
     type NodeIdentity = EndPoint
 }
