ironfleet/src/Dafny/Distributed/Services/Lock/Main.i.dfy
@@ -1,5 +1,5 @@
 include "../../Common/Framework/Main.s.dfy"
-include "../../Protocol/Lock/RefinementProof/DistributedSystem.i.dfy"
+include "LockDistributedSystem.i.dfy"
 include "../../Common/Framework/Environment.s.dfy"
 include "../../Protocol/Common/NodeIdentity.i.dfy"
 include "../../Impl/Lock/PacketParsing.i.dfy"
@@ -10,14 +10,14 @@ include "../../Protocol/Lock/RefinementProof/Refinement.i.dfy"
 include "../../Protocol/Lock/RefinementProof/RefinementProof.i.dfy"
 include "Marshall.i.dfy"
 
-module Main_i exclusively refines Main_s {
-    import opened DistributedSystem_i
+module Main_i refines Main_s {
+    import opened DS_s = Lock_DistributedSystem_i
     import opened Environment_s
     import opened Concrete_NodeIdentity_i
     import opened PacketParsing_i
     import opened UdpLock_i
     import opened Host_i
-    import opened AbstractServiceLock_s
+    import opened AS_s = AbstractServiceLock_s
     import opened Refinement_i
     import opened RefinementProof_i
     import opened MarshallProof_i
