ironfleet/src/Dafny/Distributed/Services/RSL/RSLDistributedSystem.i.dfy
@@ -1,0 +1,8 @@
+include "../../Impl/RSL/Host.i.dfy"
+include "../../Common/Framework/DistributedSystem.s.dfy"
+
+module RSL_DistributedSystem_i refines DistributedSystem_s {
+
+    import opened H_s = Host_i
+
+}
