ironfleet/src/Dafny/Libraries/Math/power.i.dfy
@@ -180,10 +180,13 @@ lemma lemma_power_auto()
 
 lemma lemma_power_positive(b:int, e:nat)
     requires 0<b;
-    ensures 0<power(b,e);
+    ensures (forall i :: i in imap u :: 0 <= u ==> 0 < power(b, u) )==> 0<power(b,e);
 {
     lemma_power_auto();
-    lemma_mul_auto_induction(e, imap u :: 0 <= u ==> 0 < power(b, u));
+    if(forall i :: i in imap u :: 0 <= u ==> 0 < power(b, u))
+    {
+        lemma_mul_auto_induction(e, imap u :: 0 <= u ==> 0 < power(b, u));
+    }
 }
 
 lemma lemma_power_increases(b:nat,e1:nat,e2:nat)
